\begin{equation}
G_C(s) = \frac{i_{\text{sv}}}{e} = \frac{i_{\text{sv}}}{x_{\text{ref}} - x_T} %= \frac{Q_L}{x_{\text{ref}} - x_T} 
\end{equation}

\begin{equation}
\left(K_q \cdot \frac{K_{\text{sv}}}{1 + \tau_{\text{sv}} s}\right) \cdot G_C(s) = \frac{Q_L}{x_{\text{ref}} - x_T} 
\end{equation}

\begin{equation}
    F_p = A \cdot P_L
\end{equation}



\begin{equation}
P_L = Q_L - A \cdot S \cdot x_T - K_c \cdot P_L
\end{equation}
\begin{equation}
P_L (1 + K_c) = Q_L - A \cdot S \cdot x_T
\end{equation}
\begin{equation}
F_p \cdot \frac{1 + K_c}{A} = \frac{K_q \cdot K_{\text{sv}} \cdot G_C(s)}{1 + \tau_{\text{sv}} \cdot s} \cdot (x_{\text{ref}} - x_T) - A \cdot S \cdot x_T \tag{1}
\end{equation}
\begin{equation}
F_p = \frac{A \cdot K_q \cdot K_{\text{sv}} \cdot G_C(s)}{(1 + K_c)(1 + \tau_{\text{sv}} \cdot s)} \cdot (x_{\text{ref}} - x_T) - \frac{S}{1 + K_c} \cdot x_T \tag{2}
\end{equation}
\begin{equation}
F_p = G_{\text{sv}} \cdot x_{\text{ref}} - \left[G_{\text{sv}} + \frac{S}{1 + K_c}\right] \cdot x_T \tag{3}
\end{equation}


\begin{equation}
 C_{sv}+\frac{s}{1+k_{c}}=\frac{A\cdot k_{q}\cdot k_{sv}\cdot C_{c}(s)+B\cdot(\lambda+\frac{1}{2}(s_{0}\cdots)}{(1+k_{0})(1+T_{sv}\cdots)} 
 \end{equation}
 
 \begin{equation}
 \frac{X_{r}}{F_{p}}=\frac{G_{1}\cdot G_{1}-G_{n}^{2}}{G_{r}\cdot G_{1}\cdot G_{1}-G_{r}\cdot E_{2}^{2}-G_{2}\cdot G_{n}^{2}}=G_{x/f_{p}}
  \end{equation}
  
 \begin{equation}
 F_{p}=C_{sv}\cdot X_{rr}-[G_{sv}+\frac{s}{1+k_{c}}]\cdot G_{sv/f_{p}}\cdot F_{p}(z)
   \end{equation}
  
 \begin{equation}
\frac{F_{p}}{x_{vr}}=\frac{G_{sv}}{1+[G_{sv}+\frac{s}{1+k_{c}}]\cdot G_{sv/f_{p}}}
\end{equation}


\begin{equation}\frac{X_{T}}{Y_{VOF}}=\frac{E_{SV}\cdot G_{N/H}}{1+E_{N/H}\cdot[E_{SV}+\frac{S}{1+N/H}]}=\frac{E_{SV}}{\frac{G_{N/H}}{G_{N/H}}+G_{SV}+\frac{S}{1+K_{C}}}\end{equation}





 %Simpletex.cn couldnt figure this one

\begin{equation}\begin{aligned}
\text{<} (1)[m_{1}\cdots^{2}+(c_{1}+c_{1})\cdots+k_{1}]\cdot X_{1}(s)=F_{p}(s)+[C_{1}\cdots+k_{1}]X_{1}(s) \\
(2)[m_{1}\cdots^{2}+(c_{1}+c_{2})\cdots+(k_{1}+k_{2})]\cdot X_{1}(s)=\underbrace{[c_{1}\cdots+k_{1}]}_{G_{1}T}X_{T}(s)+\underbrace{[c_{2}\cdots+k_{2}]}_{G_{2}T}X_{Z}(s) 
(  3)\frac{\left[m_{2}\cdots^{2}+c_{2}\cdots+k_{2}\right]\cdot X_{2}(s)}{E_{2}}=\frac{\left[c_{2}\cdots+k_{2}\right]X_{1}(s)}{G_{27}}(=)\frac{X_{2}(s)}{X_{1}(s)}=\frac{C_{2}\cdots+k_{2}}{m_{2}\cdots^{2}+C_{2}\cdots+k_{2}}=\frac{G_{22}}{G_{2}} 

\text{H} & & & & (2)=>[e_{1}]\cdot X_{1}=[e_{1}+]\cdot X_{T}+\frac{[c_{2}\cdot S+k_{2}]^{2}}{[m_{2}\cdots^{2}+c_{2}\cdots+k_{2}]}\cdot X_{1}\cdot(=)[e_{1}\cdot G_{2}-G_{2}^{2}]\cdot X_{1}=[G_{TT}\cdot G_{2}]\cdot X_{T}\Rightarrow\frac{x_{1}}{x_{T}}=\frac{G_{TT}\cdot G_{2}}{G_{T}-G_{2}^{2}} 

\Rightarrow G_{T}\cdot X_{T}=F_{P}+\frac{G_{T}^{2}\cdot G_{2}}{G_{1}\cdot G_{2}-G_{21}^{2}}\cdot X_{T}\quad(=)[G_{T}\cdot[G_{1}\cdot G_{2}-G_{21}^{2}]\div G_{T1}^{2}\cdot G_{2}]\cdot X_{T}=[G_{1}\cdot G_{2}-G_{21}^{2}]\cdot F_{P}\Rightarrow \\
 -\epsilon_{2},\epsilon_{1}^{2}
\end{aligned}\end{equation}

